experiments on the representation of ATCs

ATC.thy
@@ -48,6 +48,7 @@ where
 "
 *)
 
+(*
 datatype ('in, 'out) ATC = Leaf | Node 'in "'out \<Rightarrow> (('in, 'out) ATC)"
 
 inductive subtest :: "('in, 'out) ATC \<Rightarrow> ('in, 'out) ATC \<Rightarrow> bool" where
@@ -82,6 +83,8 @@ function atc_height :: "('in, 'out) ATC \<Rightarrow> nat" where
 "atc_height (Node x f) = Suc (Max { atc_height (f y) | y . True})"
   by pat_completeness auto
 termination by (relation subtest_rel) auto
+*)
+
 
 (*
 datatype ('in, 'out) ATC = Leaf | Node 'in "('out , (('in, 'out) ATC)) fmap"
@@ -114,7 +117,107 @@ datatype ('in, 'out) ATC = Leaf | Node 'in "('out * (('in, 'out) ATC)) list"
 
 
 
+(*
+datatype ('in, 'out) ATC = Leaf | Node 'in "('out , (('in, 'out) ATC)) fmap"
 
+inductive subtest :: "('in, 'out) ATC \<Rightarrow> ('in, 'out) ATC \<Rightarrow> bool" where
+subtest_direct : "t \<in> fmran' f \<Longrightarrow> subtest t (Node x f)" 
+
+lemma accp_subtest: "Wellfounded.accp subtest t"
+proof (induction t)
+  case Leaf
+  then show ?case by (meson ATC.distinct(1) not_accp_down subtest.simps)
+next
+  case (Node x1 x2)
+  then show ?case by (metis ATC.inject not_accp_down subtest.cases)
+qed
+
+definition subtest_rel where "subtest_rel = {(t, (Node x f)) | x f t . t \<in> fmran' f}"
+
+lemma subtest_rel_altdef: "subtest_rel = {(s, t) |s t. subtest s t}"
+  by (auto simp: subtest_rel_def subtest.simps)
+
+lemma subtest_relI [intro]: "t \<in> fmran' f \<Longrightarrow> (t, (Node x f)) \<in> subtest_rel"
+  by (simp add: subtest_rel_def)
+
+
+lemma wf_subtest_rel [simp, intro]: "wf subtest_rel"
+using accp_subtest unfolding subtest_rel_altdef accp_eq_acc wf_acc_iff
+  
+  using accp_subtest unfolding subtest_rel_altdef accp_eq_acc wf_acc_iff by sledgehamme
+*)
+(*
+datatype ('in, 'out) ATC = Leaf | Node 'in "('out , (('in, 'out) ATC)) fmap"
+fun atc_height :: "('in, 'out) ATC \<Rightarrow> nat" where
+"atc_height Leaf = 0" |
+"atc_height (Node x f) = 1 + Max ( image atc_height (fmran' f))" 
+*)
+
+datatype ('in, 'out) ATC = Leaf | Node 'in "('out , (('in, 'out) ATC)) map"
+
+fun is_atc_reaction :: "('in, 'out, 'state) FSM \<Rightarrow> 'state \<Rightarrow> ('in, 'out) ATC \<Rightarrow> ('in * 'out) list \<Rightarrow> bool" where
+"is_atc_reaction M s1 Leaf [] = True" |
+"is_atc_reaction M s1 Leaf io = False" |
+"is_atc_reaction M s1 (Node x f) [] = (\<not>(\<exists> y s2 . (s1,x,y,s2) \<in> transitions M))" | (*only relevant if M not completely specified *)
+"is_atc_reaction M s1 (Node x f) ((xi,yi)#io) = (case (f yi) of
+  Some t \<Rightarrow> (x = xi \<and> (\<exists> s2 . (s1,xi,yi,s2) \<in> transitions M \<and> is_atc_reaction M s2 t io)) |
+  None \<Rightarrow> (io = [] \<and> x = xi \<and> (\<exists> s2 . (s1,xi,yi,s2) \<in> transitions M)))"
+
+(*
+datatype ('in, 'out) ATC = Leaf | Node 'in "'out \<Rightarrow> nat" "('in, 'out) ATC list"
+
+fun atc_height :: "('in, 'out) ATC \<Rightarrow> nat" where
+"atc_height Leaf = 0" |
+"atc_height (Node x idx []) = 1" |
+"atc_height (Node x idx ts) = 1 + Max ( set (map atc_height ts)) "
+
+fun is_atc_reaction :: "('in, 'out, 'state) FSM \<Rightarrow> 'state \<Rightarrow> ('in, 'out) ATC \<Rightarrow> ('in * 'out) list \<Rightarrow> bool" where
+"is_atc_reaction M s1 Leaf [] = True" |
+"is_atc_reaction M s1 Leaf io = False" |
+"is_atc_reaction M s1 (Node x idx ts) [] = False" |
+"is_atc_reaction M s1 (Node x idx ts) ((xi,yi)#io) = (if (idx yi < length ts)
+  then (x = xi \<and> (\<exists> s2 . (s1,xi,yi,s2) \<in> transitions M \<and> is_atc_reaction M s2 (ts ! (idx yi)) io))
+  else (io = [] \<and> x = xi \<and> (\<exists> s2 . (s1,xi,yi,s2) \<in> transitions M)))" 
+*)
+
+(*
+fun atc_io :: "('in, 'out, 'state) FSM \<Rightarrow> 'state \<Rightarrow> ('in, 'out) ATC \<Rightarrow> ('in * 'out) list set" where
+"atc_io M s1 Leaf = {[]}" |
+"atc_io M s1 (Node x idx ts) = 
+  {[(x,y)] | y . \<exists> s2 . (s1,x,y,s2) \<in> transitions M \<and> idx y \<ge> length ts }
+  \<union> { (x,y)#res | y res . \<exists> s2 . (s1,x,y,s2) \<in> transitions M \<and> res \<in> atc_io M s2 (ts ! (idx y)) }"
+*)
+
+definition atc_io :: "('in, 'out, 'state) FSM \<Rightarrow> 'state \<Rightarrow> ('in, 'out) ATC \<Rightarrow> ('in * 'out) list set"
+where "atc_io M s T = { io . is_atc_reaction M s T io }"
+  
+
+lemma io_dist :
+  assumes io_diff : "act_io M s1 \<noteq> act_io M s2"
+  shows "s1 \<noteq> s2"
+  using io_diff by auto
+
+definition atc_dist :: "('in, 'out, 'state) FSM \<Rightarrow> ('in, 'out) ATC \<Rightarrow> 'state \<Rightarrow> 'state \<Rightarrow> bool" where
+"atc_dist M T s1 s2 \<equiv> atc_io M s1 T \<noteq> atc_io M s2 T"
+
+definition atc_rdist :: "('in, 'out, 'state) FSM \<Rightarrow> ('in, 'out) ATC \<Rightarrow> 'state \<Rightarrow> 'state \<Rightarrow> bool" where
+"atc_rdist M T s1 s2 \<equiv> atc_io M s1 T \<inter> atc_io M s2 T = {}"
+
+
+lemma atc_rdist_dist :
+  assumes wf1 : "well_defined M1"
+  assumes wf2 : "well_defined M2"
+  assumes ob1 : "observable M1"
+  assumes ob2 : "observable M2"
+  assumes el_s1 : "s1 \<in> states M1"
+  assumes el_s2 : "s2 \<in> states M1"
+  assumes el_t1 : "t1 \<in> states M2"
+  assumes el_t2 : "t2 \<in> states M2"
+  assumes red1 : "io_reduction_state M2 t1 M1 s1"
+  assumes red2 : "io_reduction_state M2 t2 M1 s2"
+  assumes rdist: "atc_rdist M1 T s1 s2"
+  shows "atc_dist M2 T t1 t2"
+  oops
 
 
 
